[C2C] Adapt and improve proof generation.
The adaptation is for the extension of `exec-expr` to handle unary expressions
that may not be pure. The improvement pertains to some generalizations that will
be useful for future extensions.

books/kestrel/c/transformation/proof-generation-theorems.lisp
@@ -12,12 +12,55 @@
 
 (include-book "proof-generation")
 
+(include-book "../atc/pure-expression-limits")
+
 (include-book "std/util/defund-sk" :dir :system)
 
 (local (include-book "kestrel/built-ins/disable" :dir :system))
 (local (acl2::disable-most-builtin-logic-defuns))
 (local (acl2::disable-builtin-rewrite-rules-for-defaults))
 (set-induction-depth-limit 0)
+
+;;;;;;;;;;;;;;;;;;;;;;;;;;;;;;;;;;;;;;;;;;;;;;;;;;;;;;;;;;;;;;;;;;;;;;;;;;;;;;;;
+
+; move to C formalization:
+
+(local
+ (defun induction (expr limit)
+   (declare (xargs :measure (c::expr-count expr)
+                   :hints (("Goal" :in-theory (enable o< o-finp)))))
+   (declare (irrelevant limit))
+   (c::expr-case expr
+                 :ident nil
+                 :const nil
+                 :call nil
+                 :unary (induction expr.arg (1- limit))
+                 :otherwise nil)))
+
+(defruled c::exec-expr-to-exec-expr-pure
+  (implies (and (c::expr-purep expr)
+                (>= (nfix limit) (c::expr-pure-limit expr)))
+           (equal (c::exec-expr expr compst fenv limit)
+                  (mv (c::exec-expr-pure expr compst)
+                      (c::compustate-fix compst))))
+  :induct (induction expr limit)
+  :expand (c::exec-expr-pure expr compst)
+  :enable (c::exec-expr
+           c::expr-pure-limit
+           c::expr-purep
+           nfix))
+
+(defruled pure-limit-bound-when-exec-expr-not-error
+  (b* (((mv eval &) (c::exec-expr expr compst fenv limit)))
+    (implies (and (c::expr-purep expr)
+                  (not (c::errorp eval)))
+             (>= (nfix limit) (c::expr-pure-limit expr))))
+  :rule-classes ((:linear :trigger-terms ((c::expr-pure-limit expr))))
+  :induct (induction expr limit)
+  :enable (c::exec-expr
+           c::expr-pure-limit
+           c::expr-purep
+           nfix))
 
 ;;;;;;;;;;;;;;;;;;;;;;;;;;;;;;;;;;;;;;;;;;;;;;;;;;;;;;;;;;;;;;;;;;;;;;;;;;;;;;;;
 
@@ -107,7 +150,28 @@
      we use potentially different function environments
      for the old vs. new constructs.
      We always use the same initial computation state
-     for old and new constructs."))
+     for old and new constructs.")
+   (xdoc::p
+    "The theorem @('expr-pure-congruence') is a bit different,
+     because it does not change the expressions,
+     but it changes from @(tsee c::exec-expr-pure) to @(tsee c::exec-expr).
+     So it is still a form of equivalence lifting,
+     and it has a form similar to other theorems.
+     A critical hypothesis is that the limit for the new expression
+     does not exceed the limit for the old expression:
+     this is so that, under the assumption that the old expression
+     does not yield an error under @(tsee c::exec-expr),
+     neither does the new expression.
+     In the absence of this hypothesis,
+     the new expression could need a higher limit.
+     In general, transformations may need to also transform limits;
+     for now these theorems support transformations in which
+     the limit does not increase,
+     but we plan to generalize this.")
+   (xdoc::p
+    "The same hypothesis on pure expression limits is also in
+     @('initer-single-pure-congruence') and @('stmt-return-value-congruence'),
+     because they also involve lifting from pure expressions."))
 
   ;;;;;;;;;;;;;;;;;;;;;;;;;;;;;;;;;;;;;;;;
 
@@ -564,25 +628,36 @@
 
   ;;;;;;;;;;;;;;;;;;;;;;;;;;;;;;;;;;;;;;;;
 
-  (defruled exec-expr-when-exec-expr-pure-integer
-    (b* ((expr-result (c::exec-expr-pure expr compst))
-         (expr-value (c::expr-value->value expr-result))
-         (type (c::type-of-value expr-value)))
-      (implies (and (c::expr-purep expr)
-                    (not (c::errorp expr-result))
-                    (c::type-nonchar-integerp type)
-                    (not (zp limit)))
-               (equal (c::exec-expr expr compst fenv limit)
-                      (mv expr-result (c::compustate-fix compst)))))
-    :use ((:instance c::not-call-when-exec-expr-pure-not-error
-                     (expr expr) (compst compst))
-          (:instance c::not-asg-when-exec-expr-pure-not-error
-                     (expr expr) (compst compst)))
-    :enable (c::exec-expr
-             c::exec-expr-pure
-             c::apconvert-expr-value-when-not-array
-             c::value-kind-not-array-when-value-integerp
-             c::expr-valuep-when-expr-value-resultp-and-not-errorp))
+  (defruled expr-pure-congruence
+    (b* ((old-eval-pure (c::exec-expr-pure old compst))
+         (new-eval-pure (c::exec-expr-pure new compst))
+         (old-val-pure (c::expr-value->value old-eval-pure))
+         (new-val-pure (c::expr-value->value new-eval-pure))
+         ((mv old-eval old-compst) (c::exec-expr old compst old-fenv limit))
+         ((mv new-eval new-compst) (c::exec-expr new compst new-fenv limit))
+         (old-val (c::expr-value->value old-eval))
+         (new-val (c::expr-value->value new-eval)))
+      (implies (and (c::expr-purep old)
+                    (c::expr-purep new)
+                    (not (c::errorp old-eval))
+                    (not (c::errorp new-eval-pure))
+                    (equal old-val-pure new-val-pure)
+                    (<= (c::expr-pure-limit new) (c::expr-pure-limit old)))
+               (and (not (c::errorp new-eval))
+                    (iff old-eval new-eval)
+                    (equal old-val new-val)
+                    (equal old-compst new-compst)
+                    (equal (c::type-of-value old-val)
+                           (c::type-of-value old-val-pure)))))
+    :use ((:instance c::exec-expr-to-exec-expr-pure
+                     (expr old)
+                     (fenv old-fenv))
+          (:instance c::exec-expr-to-exec-expr-pure
+                     (expr new)
+                     (fenv new-fenv)))
+    :enable (pure-limit-bound-when-exec-expr-not-error
+             nfix
+             c::exec-expr))
 
   ;;;;;;;;;;;;;;;;;;;;;;;;;;;;;;;;;;;;;;;;
 
@@ -600,6 +675,8 @@
          (type (c::type-of-value old-expr-value)))
       (implies (and (c::expr-purep old-expr)
                     (c::expr-purep new-expr)
+                    (<= (c::expr-pure-limit new-expr)
+                        (c::expr-pure-limit old-expr))
                     (not (c::errorp old-result))
                     (not (c::errorp new-expr-result))
                     (equal old-expr-value new-expr-value)
@@ -610,12 +687,10 @@
                     (equal (c::init-type-of-init-value old-result)
                            (c::init-type-single type)))))
     :expand ((c::exec-initer (c::initer-single old-expr) compst old-fenv limit)
-             (c::exec-initer (c::initer-single new-expr) compst new-fenv limit)
-             (c::exec-expr old-expr compst old-fenv (+ -1 limit))
-             (c::exec-expr new-expr compst new-fenv (+ -1 limit)))
-    :enable (c::exec-expr
-             c::exec-expr-pure
-             c::expr-purep
+             (c::exec-initer (c::initer-single new-expr) compst new-fenv limit))
+    :enable (c::exec-expr-to-exec-expr-pure
+             pure-limit-bound-when-exec-expr-not-error
+             nfix
              c::apconvert-expr-value-when-not-array
              c::value-kind-not-array-when-value-integerp
              c::init-type-of-init-value))
@@ -677,6 +752,8 @@
                     new-expr
                     (c::expr-purep old-expr)
                     (c::expr-purep new-expr)
+                    (<= (c::expr-pure-limit new-expr)
+                        (c::expr-pure-limit old-expr))
                     (not (c::errorp old-result))
                     (not (c::errorp new-expr-result))
                     (iff old-expr-result new-expr-result)
@@ -690,12 +767,10 @@
                     (set::in (c::type-option-of-stmt-value old-result)
                              (set::insert type nil)))))
     :expand ((c::exec-stmt (c::stmt-return old-expr) compst old-fenv limit)
-             (c::exec-stmt (c::stmt-return new-expr) compst new-fenv limit)
-             (c::exec-expr old-expr compst old-fenv (+ -1 limit))
-             (c::exec-expr new-expr compst new-fenv (+ -1 limit)))
-    :enable (c::exec-expr
-             c::exec-expr-pure
-             c::expr-purep
+             (c::exec-stmt (c::stmt-return new-expr) compst new-fenv limit))
+    :enable (c::exec-expr-to-exec-expr-pure
+             pure-limit-bound-when-exec-expr-not-error
+             nfix
              c::type-of-value
              c::apconvert-expr-value-when-not-array
              c::type-nonchar-integerp
@@ -1206,17 +1281,23 @@
 
   ;;;;;;;;;;;;;;;;;;;;;;;;;;;;;;;;;;;;;;;;
 
+  (defruled expr-pure-errors
+    (implies (and (c::expr-purep expr)
+                  (c::errorp (c::exec-expr-pure expr compst)))
+             (c::errorp (mv-nth 0 (c::exec-expr expr compst fenv limit))))
+    :use c::exec-expr-to-exec-expr-pure
+    :enable pure-limit-bound-when-exec-expr-not-error)
+
+  ;;;;;;;;;;;;;;;;;;;;;;;;;;;;;;;;;;;;;;;;
+
   (defruled initer-single-pure-errors
     (implies (and (c::expr-purep expr)
                   (c::errorp (c::exec-expr-pure expr compst)))
              (c::errorp
               (mv-nth 0 (c::exec-initer
                          (c::initer-single expr) compst fenv limit))))
-    :expand ((c::exec-initer (c::initer-single expr) compst fenv limit)
-             (c::exec-expr expr compst fenv (+ -1 limit)))
-    :enable (c::exec-expr
-             c::exec-expr-pure
-             c::expr-purep))
+    :expand (c::exec-initer (c::initer-single expr) compst fenv limit)
+    :enable expr-pure-errors)
 
   ;;;;;;;;;;;;;;;;;;;;;;;;;;;;;;;;;;;;;;;;
 
@@ -1239,11 +1320,8 @@
                                       compst
                                       fenv
                                       limit))))
-    :expand ((c::exec-stmt (c::stmt-return expr) compst fenv limit)
-             (c::exec-expr expr compst fenv (+ -1 limit)))
-    :enable (c::exec-expr
-             c::exec-expr-pure
-             c::expr-purep))
+    :expand (c::exec-stmt (c::stmt-return expr) compst fenv limit)
+    :enable expr-pure-errors)
 
   ;;;;;;;;;;;;;;;;;;;;;;;;;;;;;;;;;;;;;;;;
 
